set up for buggy zk proof

ironfleet/src/Dafny/Distributed/Protocol/ZooKeeper/PerformamceProof/BuggyZKInvariants.dfy
@@ -43,4 +43,112 @@ predicate EmptyDiff_Invariant(tls:TLS_State) {
         && !pkt.msg.v.SyncTRUNC?
         && !pkt.msg.v.Commit?
 }
+
+
+predicate EmptyDiff_Invariant_Inductive(tls:TLS_State) 
+    requires DS_Config_Invariant(tls.config, tls)
+    requires ZK_Config_Invariant(tls.config, tls)
+    requires |tls.initialZkdbState| == |tls.config|
+{
+    && EmptyDiff_Invariant(tls)
+    && Dbs_Are_Identical(tls)
+    && All_Messages_Have_Same_Zxid(tls)
+    && Leader_Have_Bad_Zxid(tls)
+    && Leader_Only_Send_SyncSnap(tls)
+}
+
+predicate Dbs_Are_Identical(tls:TLS_State) 
+    requires DS_Config_Invariant(tls.config, tls)
+    requires ZK_Config_Invariant(tls.config, tls)
+    requires |tls.initialZkdbState| == |tls.config|
+{
+    var target_db := tls.initialZkdbState[0];
+    var target_zxid := getLastLoggedZxid(target_db);
+    tls.t_servers[tls.config[0]].v.leader.globals.zkdb.commitLog == target_db.commitLog
+    && (forall ep | ep in tls.t_servers && tls.t_servers[ep].v.FollowerPeer?
+        ::
+        tls.t_servers[ep].v.follower.zkdb.commitLog == target_db.commitLog)
+}
+
+predicate All_Messages_Have_Same_Zxid(tls:TLS_State) 
+    requires DS_Config_Invariant(tls.config, tls)
+    requires ZK_Config_Invariant(tls.config, tls)
+    requires |tls.initialZkdbState| == |tls.config|
+{
+    var target_db := tls.initialZkdbState[0];
+    var target_zxid := getLastLoggedZxid(target_db);
+    forall pkt | pkt in tls.t_environment.sentPackets ::
+    && (pkt.msg.v.FollowerInfo? ==> pkt.msg.v.latestZxid == target_zxid) 
+    && (pkt.msg.v.AckEpoch? ==> pkt.msg.v.lastLoggedZxid == target_zxid) 
+}
+
+predicate Leader_Have_Bad_Zxid(tls:TLS_State) 
+    requires DS_Config_Invariant(tls.config, tls)
+    requires ZK_Config_Invariant(tls.config, tls)
+    requires |tls.initialZkdbState| == |tls.config|
+{
+    var target_db := tls.initialZkdbState[0];
+    var target_zxid := getLastLoggedZxid(target_db);
+    var l := tls.t_servers[tls.config[0]].v.leader;
+    forall h | h in l.handlers ::
+        && (l.handlers[h].peerLastZxid != NullZxid ==> l.handlers[h].peerLastZxid == target_zxid)
+        && (l.handlers[h].peerLastZxid != NullZxid ==> l.globals.currZxid == Zxid(l.globals.leaderEpoch, 0))
+        && (l.handlers[h].peerLastZxid != NullZxid ==> l.handlers[h].peerLastZxid != l.globals.currZxid)
+}
+
+predicate Leader_Only_Send_SyncSnap(tls:TLS_State) 
+    requires DS_Config_Invariant(tls.config, tls)
+    requires ZK_Config_Invariant(tls.config, tls)
+    requires |tls.initialZkdbState| == |tls.config|
+{
+    var l := tls.t_servers[tls.config[0]].v.leader;
+    forall h | h in l.handlers ::
+        forall p | p in l.handlers[h].queuedPackets :: p.SyncSNAP?
+}
+
+
+
+/* Main theorem */
+lemma theorem_ZK_Buggy_Guarantee(config:Config, tlb:seq<TLS_State>, f:int)
+    requires |tlb| > 1
+    requires SeqIsUnique(config);
+    requires ValidTLSBehavior(config, tlb, f)
+    requires Performance_Assumption_EmptyDiff(tlb)
+    requires forall i | 0 <= i < |tlb| :: Basic_Invariants(config, tlb[i])
+    ensures forall i | 0 <= i < |tlb| :: |tlb[i].initialZkdbState| == |config|
+    ensures forall i | 0 <= i < |tlb| :: EmptyDiff_Invariant(tlb[i])
+{
+    assert |tlb[0].initialZkdbState| == |config|;
+    assert EmptyDiff_Invariant_Inductive(tlb[0]);
+    var i := 0;
+    while i < |tlb| - 1 
+        decreases |tlb| - i
+        invariant 0 <= i < |tlb|
+        invariant forall k | 0 <= k <= i :: |tlb[k].initialZkdbState| == |config|
+        invariant forall k | 0 <= k <= i :: EmptyDiff_Invariant_Inductive(tlb[k])
+    {   
+        var tls, tls' := tlb[i], tlb[i+1];
+        theorem_ZK_Buggy_Guarantee_Induction(config, tls, tls', f);
+        assert EmptyDiff_Invariant_Inductive(tls');
+        i := i + 1;
+    }
+}
+
+
+/* Main theorem */
+lemma theorem_ZK_Buggy_Guarantee_Induction(config:Config, tls:TLS_State, tls':TLS_State, f:int)
+    requires TLS_Next(tls, tls')
+    requires Basic_Invariants(config, tls) && Basic_Invariants(config, tls')
+    requires |tls.initialZkdbState| == |config|
+    requires EmptyDiff_Invariant_Inductive(tls)
+    ensures |tls'.initialZkdbState| == |config|
+    ensures EmptyDiff_Invariant_Inductive(tls')
+{
+    assert Dbs_Are_Identical(tls');
+    assert All_Messages_Have_Same_Zxid(tls');
+    assert Leader_Have_Bad_Zxid(tls');
+    assert Leader_Only_Send_SyncSnap(tls');
+    assert EmptyDiff_Invariant(tls');
+}
+
 }
